More progress

verified/sec_prop.i.dfy
@@ -1,88 +1,21 @@
-include "smcapi.s.dfy"
-include "pagedb.i.dfy"
-include "ptables.i.dfy"
+include "sec_prop.s.dfy"
+include "pagedb.s.dfy"
+include "entry.s.dfy"
 
-/* 
- * If I recall correctly these exist / existed elsewhere... dig later
- */
-predicate valAddrPage(d: PageDb, n: PageNr)
-    requires validPageDb(d)
+
+lemma enter_enc_enc_conf_ni(s1: state, d1: PageDb, s1':state, d1': PageDb,
+                            s2: state, d2: PageDb, s2':state, d2': PageDb,
+                    dispPage: word, arg1: word, arg2: word, arg3: word)
+    requires SaneState(s1) && validPageDb(d1) && SaneState(s1') && validPageDb(d1')
+    requires SaneState(s2) && validPageDb(d2) && SaneState(s2') && validPageDb(d2')
+    requires pageDbCorresponds(s1.m, d1) && pageDbCorresponds(s1'.m, d1') 
+    requires pageDbCorresponds(s1.m, d2) && pageDbCorresponds(s2'.m, d2') 
+    requires validPageNr(dispPage) && valDispPage(d1, dispPage) // Error case??
+    requires smc_enter(s1, d1, s1', d1', dispPage, arg1, arg2, arg3)
+    requires smc_enter(s2, d2, s2', d2', dispPage, arg1, arg2, arg3)
+    requires enc_enc_conf_eqpdb(d1, d2, dispPage)
+    requires enc_enc_conf_eq(s1, s2, d1, d2, dispPage)
+    ensures  enc_enc_conf_eqpdb(d1', d2', dispPage)
+    ensures  enc_enc_conf_eq(s1', s2', d1', d2', dispPage)
 {
-    d[n].PageDbEntryTyped? && d[n].entry.Addrspace?
-}
-
-predicate pgInAddrSpc(d: PageDb, n: PageNr, a: PageNr)
-    requires validPageDb(d) && valAddrPage(d, a)
-{
-    d[n].PageDbEntryTyped? && d[n].addrspace == a
-}
-
-// I am not sure if we have a well-defined notion of an "enclave number" aside 
-// from an addrspace page, so I am using addrspace pages as an enclave number 
-// in this file.
-
-// Should be true if the enclave in addrspace a is currently executing.
-// I'm not sure if we have a better way of testing whether or not an enclave is 
-// currently executing.
-predicate isEncExecuting(s:state, d:pagedb, a:PageNr)
-    requires SaneState(s) && validPageDb(d) && pageDbCorresponds(s, d)
-    requires valAddrPage(d, a)
-{
-    s.conf.ttbr0.ptbase == page_paddr(l1p)
-}
-
-//-----------------------------------------------------------------------------
-// Protect confidentiality of an Enclave from other Enclaves 
-//-----------------------------------------------------------------------------
-// A malicious enclave can observe:
-// 1. Pages it owns.
-// 2. Public pages.
-// 3. Registers *only* when the malicious enclave is executing.
-
-// Low-equivalence relation that relates two PageDbs that appear equivalent to 
-// an attacker that controls an enclave in addrspace "atkr". 
-predicate enc_enc_conf_eqpdb(d1:pagedb, d2: pagedb, atkr:PageNr)
-    requires validPageDb(d1) && validPageDb(d2)
-    requires valAddrPage(d1, atkr)
-{
-    valAddrPage(d2, atkr) &&
-    (forall n : PageNr :: pgInAddrSpc(d1, n, atkr) <==>
-        pgInAddrSpc(d2, n, atkr)) &&
-    (forall n : PageNr | pgInAddrSpc(d1, n, atkr) ::
-        d2[n].PageDbEntryTyped? && d1[n].entry == d2[n].entry)
-}
-
-// Low-equivalence relation that relates two concrete states that appear 
-// equivalent to an attacker that controls an enclave in adddrspace "atkr". 
-// A malicous attacker cannot observe anything when it is not executing (but it 
-// can always observe whether or not it is executing).
-predicate enc_enc_conf_eq(s1:state, s2:state, d1:pagedb, d2:pagedb, 
-    atkr:PageNr)
-    requires SaneState(s1) && SaneState(s2)
-    requires validPageDb(d1) && validPageDb(d2)
-    requires pageDbCorresponds(s1.m, d1) && pageDbCorresponds(s2.m, d2)
-    requires valAddrPage(d1, atkr)
-    requires enc_enc_conf_eqpdb(d1, d2, atkr)
-{
-    var l1p := d1[atkr].entry.l1ptnr // same in both d1, d2 because of precond
-    (isEncExecuting(s1, d1, atkr) <==> isEncExecuting(s2, d2, atkr)) &&
-    (isEncExecuting(s1, d1, atkr) ==>
-        s1.regs == s2.regs &&
-        s1.sregs == s2.sregs &&
-        PagsInTable(mkAbsPTable(d1, l1p)) == 
-            PagsInTable(mkAbsPTable(d2, l1p))
-    )
-
-}
-
-// Like WritablePagesInTable but includes pages without the write bit set
-
-function PagesInTable(pt:AbsPTable): set<addr>
-    requires WellformedAbsPTable(pt)
-    ensures forall m:addr :: m in WritablePagesInTable(pt) ==> PageAligned(m)
-{
-    (set i, j | 0 <= i < |pt| && pt[i].Just? && 0 <= j < |pt[i].v|
-        && pt[i].v[j].Just?
-        :: (assert WellformedAbsPTE(pt[i].v[j]);
-          pt[i].v[j].v.phys + PhysBase()))
 }
