verified/sec_prop.s.dfy
@@ -1,0 +1,121 @@
+include "smcapi.s.dfy"
+//include "pagedb.i.dfy"
+include "pagedb.s.dfy"
+// I need this until we figure out how to extract just the trusted parts
+include "ptables.i.dfy"
+
+/* 
+ * If I recall correctly these exist / existed elsewhere... dig later
+ */
+predicate valDispPage(d: PageDb, n: PageNr)
+    requires validPageDb(d)
+{
+    d[n].PageDbEntryTyped? && d[n].entry.Dispatcher?
+}
+
+predicate valAddrPage(d: PageDb, n: PageNr)
+    requires validPageDb(d)
+{
+    d[n].PageDbEntryTyped? && d[n].entry.Addrspace?
+}
+
+predicate pgInAddrSpc(d: PageDb, n: PageNr, a: PageNr)
+    requires validPageDb(d) && valAddrPage(d, a)
+{
+    d[n].PageDbEntryTyped? && d[n].addrspace == a
+}
+
+predicate pgInEnc(d: PageDb, n: PageNr, enc: PageNr)
+    requires validPageDb(d) && valDispPage(d, enc)
+{
+    d[n].PageDbEntryTyped? && (d[n].addrspace == d[enc].addrspace)
+}
+
+//-----------------------------------------------------------------------------
+// Protect confidentiality of an Enclave from other Enclaves 
+//-----------------------------------------------------------------------------
+// A malicious enclave can observe:
+// 1. Pages it owns.
+// 2. Public pages.
+// 3. (A subset of the) registers *only* when the malicious enclave is executing.
+
+// Low-equivalence relation that relates two PageDbs that appear equivalent to 
+// an attacker that controls an enclave in addrspace "atkr". 
+predicate enc_enc_conf_eqpdb(d1:PageDb, d2: PageDb, atkr:PageNr)
+    requires validPageDb(d1) && validPageDb(d2)
+    requires valDispPage(d1, atkr)
+{
+    var atkr_asp := d1[atkr].addrspace;
+    valDispPage(d2, atkr) &&
+    d1[atkr].addrspace == d2[atkr].addrspace &&
+    valAddrPage(d1, atkr) && valAddrPage(d2, atkr) &&
+    (forall n : PageNr :: pgInAddrSpc(d1, n, atkr) <==>
+        pgInAddrSpc(d2, n, atkr)) &&
+    (forall n : PageNr | pgInAddrSpc(d1, n, atkr) ::
+        d2[n].PageDbEntryTyped? && d1[n].entry == d2[n].entry)
+}
+
+// Low-equivalence relation that relates two concrete states that appear 
+// equivalent to an attacker that controls an enclave in adddrspace "atkr". 
+// A malicous attacker cannot observe anything when it is not executing (but it 
+// can always observe whether or not it is executing).
+//
+// The plan is to only check low-equivalence of states on entry/exit of 
+// the enclave so this only needs to hold then.
+predicate enc_enc_conf_eq(s1:state, s2:state, d1:PageDb, d2:PageDb, 
+    atkr:PageNr)
+    requires SaneState(s1) && SaneState(s2)
+    requires validPageDb(d1) && validPageDb(d2)
+     requires pageDbCorresponds(s1.m, d1) && pageDbCorresponds(s2.m, d2)
+    requires valDispPage(d1, atkr)
+    requires valAddrPage(d1, d1[atkr].addrspace)
+    requires enc_enc_conf_eqpdb(d1, d2, atkr)
+{
+    var atkr_asp := d1[atkr].addrspace;
+    var l1p := d1[atkr_asp].entry.l1ptnr; // same in both d1, d2 because of eqdb
+    regs_usr_equiv(s1.regs, s2.regs) &&
+    configs_usr_equiv(s1.conf, s2.conf) &&
+    nonStoppedL1(d1, l1p) ==>
+        (PagesInTable(mkAbsPTable(d1, l1p)) == 
+            PagesInTable(mkAbsPTable(d2, l1p)))
+
+}
+
+predicate regs_usr_equiv(r1:map<ARMReg,word>, r2:map<ARMReg,word>)
+    requires ValidRegState(r1) && ValidRegState(r2)
+{
+    reveal_ValidRegState();
+    r1[R0]  == r2[R0] &&
+    r1[R1]  == r2[R1] &&
+    r1[R2]  == r2[R2] &&
+    r1[R3]  == r2[R3] &&
+    r1[R4]  == r2[R4] &&
+    r1[R5]  == r2[R5] &&
+    r1[R6]  == r2[R6] &&
+    r1[R7]  == r2[R7] &&
+    r1[R8]  == r2[R8] &&
+    r1[R9]  == r2[R9] &&
+    r1[R10] == r2[R10] &&
+    r1[R11] == r2[R11] &&
+    r1[R12] == r2[R12] &&
+    r1[SP(User)] == r2[SP(User)] &&
+    r1[LR(User)] == r2[LR(User)]
+}
+
+predicate configs_usr_equiv(c1:config, c2:config)
+{
+    // AFAIK nothing is visible in usermode
+    true
+}
+
+// Like WritablePagesInTable but includes pages without the write bit set
+
+function PagesInTable(pt:AbsPTable): set<addr>
+    requires WellformedAbsPTable(pt)
+    ensures forall m:addr :: m in WritablePagesInTable(pt) ==> PageAligned(m)
+{
+    (set i, j | 0 <= i < |pt| && pt[i].Just? && 0 <= j < |pt[i].v|
+        && pt[i].v[j].Just?
+        :: (assert WellformedAbsPTE(pt[i].v[j]);
+          pt[i].v[j].v.phys + PhysBase()))
+}
